Tuple hacked

Cpc/Spec.lean
@@ -369,7 +369,10 @@ def __eo_to_smt : Term -> SmtTerm
   | (Term.Apply (Term.Apply (Term.UOp UserOp.is) x1) x2) => (SmtTerm.Apply (__eo_to_smt_tester (__eo_to_smt x1)) (__eo_to_smt x2))
   | (Term.Apply (Term.Apply (Term.Apply (Term.UOp UserOp.update) x1) x2) x3) => (__eo_to_smt_updater (__eo_to_smt x1) (__eo_to_smt x2) (__eo_to_smt x3))
   | (Term.UOp UserOp.tuple_unit) => (SmtTerm.DtCons "_at_Tuple" (SmtDatatype.sum SmtDatatypeCons.unit SmtDatatype.null) native_nat_zero)
-  | (Term.Apply (Term.Apply (Term.UOp UserOp.tuple) x1) x2) => (SmtTerm.Apply (__eo_to_smt_tuple_app_extend (__eo_to_smt x1) (__eo_to_smt_type (__eo_typeof x2))) (__eo_to_smt x2))
+  | (Term.Apply (Term.Apply (Term.UOp UserOp.tuple) x1) x2) =>
+    let _v0 := (SmtTerm.Apply (__eo_to_smt_tuple_app_extend (__eo_to_smt x1) (__eo_to_smt_type (__eo_typeof x2))) (__eo_to_smt x2))
+    let _v1 := (__eo_to_smt_type (__eo_typeof (Term.Apply (Term.Apply (Term.UOp UserOp.tuple) x1) x2)))
+    (native_ite (native_Teq (__smtx_typeof _v0) _v1) _v0 SmtTerm.None)
   | (Term.Apply (Term.Apply (Term.UOp UserOp.tuple_select) x1) x2) => (__eo_to_smt_tuple_select (__eo_to_smt_type (__eo_typeof x2)) (__eo_to_smt x1) (__eo_to_smt x2))
   | (Term.Apply (Term.Apply (Term.Apply (Term.UOp UserOp.tuple_update) x1) x2) x3) => (__eo_to_smt_tuple_update (__eo_to_smt_type (__eo_typeof x2)) (__eo_to_smt x1) (__eo_to_smt x2) (__eo_to_smt x3))
   | (Term.set_empty x1) => (__eo_to_smt_set_empty (__eo_to_smt_type x1))
